---
title: 'IMO 2012 Problem 2 - Solution'
date: 2021-03-20
permalink: /posts/2021/03/imo-2012-problem-02-solution/
tags:
  - maths
  - imo
  - inequation
  - am-gm
---

Let's play with the 2nd problem of the International Mathematics Olympiad (IMO) 2012.

## Problem

For `n >= 3` where `n` is an integer and `A2, ..., An` are positive real numbers and `A2 . A3 . ... . An = 1`, prove the following:

`(1 + A2)^2 . (1 + A3)^3 . (1 + A4)^4 . ... . (1 + An)^n > n^n`.

---

## Solution

For this problem, we're going to leverage AM-GM inequality which states `(X1 + X2 + ... + Xn) / n >= n-root(X1 . X2 . X3 ... Xn)`.

Starting with a small step, we'll see what the form of AM-GM is for `(1 + A2)`. Based on the AM-GM formula, the inequality form of `(1 + A2)` will be `(1 + A2) / 2 >= sqrt(A2)`.

However, the trick lies on how we express `1` within `(1 + An)`. Precisely, for `2 <= m <= n`, we can rewrite `(1 + Am)` as `((1 / (m-1)) * (m-1) + Am)`. Note that we replace `1` with `1 / (m-1)` which repeated `m-1` times.

With the above in mind, let's apply the AM-GM form for `(1 + Am)` where `2 <= m <= n`.

```
[1 / (m-1) + 1 / (m-1) + ... + Am] / m >= m-root(Am / (m-1)^m-1)
```

Move the denominator `m` from LHS to RHS which yields the following.

```
[1 / (m-1) + 1 / (m-1) + ... + Am] >= m . m-root(Am / (m-1)^m-1)
```

Take the power of `m` for both LHS and RHS.

```
[1 / (m-1) + 1 / (m-1) + ... + Am]^m >= m^m . (Am / (m-1)^m-1)
```

From the last inequation above, we could rewrite it as `[1 + Am]^m >= m^m . (Am / (m-1)^m-1)`.

Next, multiply the LHS with `(1 + Am)^m` where `m` starts from `2` until `n` such as the following.

```
(1+A2)^2 . (1+A3)^3 . (1+A4)^4 . ... . (1+An)^n
```

The same thing also applies to the RHS. Note that the inequality sign doesn't change.

```
2^2 . (A2) . 3^3 . (A3 / 2^2) . 4^4 . (A4 / 3^3) . ... . n^n . (An / (n-1)^n-1)
```

From the RHS, it's clear that we can eliminate `2^2, 3^3, 4^4, ..., (n-1)^n-1` and the remaining terms are `A2 . A3 . A4 . ... . An . n^n`.

Since we know from the problem statement that `A2 . A3 . A4 . ... . An` equals to 1, then the RHS has only `n^n` as its term. In other words, we got `(1 + A2)^2 . (1 + A3)^3 . (1 + A4)^4 . ... . (1 + An)^n >= n^n`.

However, our proof has not completed yet since the inequality sign is still `>=` instead of `>`.

Note that equality holds when `(1 + Am)^m = m^m . (Am / (m-1)^m-1)` for `2 <= m <= n`.

From the AM-GM form of `(1 + Am)`, we know that the equality holds when `Am` equals to `1 / (m-1)`.

Take a look at the following.

```
[1 / (m-1) + 1 / (m-1) + ... + Am] / m >= m-root(Am / (m-1)^m-1)

Both LHS and RHS will be equal when Am = 1 / (m-1) as shown below.

1 / (m-1) = m-root(1 / (m-1)^m)
1 / (m-1) = 1 / (m-1)
```

However, when `Am` equals to `1 / (m-1)`, the expression `A2 . A3 . A4 . ... . An` will return `1 . 1 / 2 . 1 / 3 . ... . 1 / (n-1)` or `1 / (n-1)!` which cannot be 1. This happens because `n >= 3` according to the problem statement.

Therefore, equality cannot hold and we can discard the equal sign from `>=`. Finally, we end up with the following.

```
`(1 + A2)^2 . (1 + A3)^3 . (1 + A4)^4 . ... . (1 + An)^n > n^n`
```

Q.E.D
